\documentclass{../templetes/1c}
\usepackage{graphicx}
\usepackage{bm}

\begin{document}
\title {Diffusion-convection equation in 2d plane}
\date{\today}
\maketitle

The diffusion-convection equation reads

\begin{equation}
D\nabla^2g+\nabla\cdot(\frac{\bm{f}}{\gamma_0}g)
+\nabla\cdot(\bm{u}g)=0
\end{equation}
with boundary condition
\begin{equation}
g(r\rightarrow\infty )=1
\end{equation}

For simplicity, set $\gamma_0=D=1
$.


\section{Plane Geometry}

\begin{equation} \label{p}
\pd_x^2g+\pd_x[-(\pd_xV)g]
+U_x\pd_xg+\pd_y^2g+\pd_y[-(\pd_yV)g]+U_y\pd_yg=0
\end{equation}
with BC
\begin{equation}
g(r\rightarrow\infty)=1
\end{equation}

The potential is
\begin{equation}
V(x,y)=\frac{K}{2}(x^2+y^2)=v(x)v(y), \mbox{ with } v(x)=\frac{K}{2}x^2.
\end{equation}

\subsection{Separation of variables(NOT appliable!)}
Eq.\eqref{p} may be solved by separating the varibles as $g(x,y)=F(x)W(y)$.
So Eq.\eqref{p} is transformed to

\begin{equation}
    WF''+Wv_y(-v_x'F)'+WU_xF'+
    FW''+FU_yW'+Fv_y(-v_y'W)'=0
\end{equation}
However, the above eq. can not be seprated.
Noting that

\begin{equation}
    F''/F+v_y(-v_x'F)'/F+U_xF'/F+
    W''/W+U_yW'/W+v_y(-v_y'W)'/W=0
\end{equation}
Due to interaction, the term $v_y(-v_x'F)'$
still depends on $y$. Physically, the equation is
not separable because the interaction couples the
equation in different dimensions.



\end{document}



Let $g=1+e^{-\lambda x}w(r,\theta)$
We have
\begin{equation}
\pd_x g=-\lambda e^{-\lambda x}w+e^{-\lambda x}\pd_xw
\end{equation}

\begin{equation}
\pd_x^2 g=\lambda^2 e^{-\lambda x}w-2\lambda e^{-\lambda x}\pd_xw+
e^{-\lambda x}\pd_x^2w
\end{equation}

\begin{equation}
\pd_y^2 g=e^{-\lambda x}\pd_y^2 w
\end{equation}

so
\begin{equation}
\nabla^2 g=\lambda^2 e^{-\lambda x}w-2\lambda e^{-\lambda x}\pd_xw+
e^{-\lambda x}\nabla^2w
\end{equation}

and

\begin{equation}
U\pd_xg=
-U\lambda e^{-\lambda x}w+
Ue^{-\lambda x}\pd_xw
\end{equation}

To cancel the term $\pd_x w$
let $\lambda=\frac{U}{2}$.

So
\begin{equation}
\nabla^2 g+U\pd_xg=e^{-\lambda x}(-\frac{U^2}{4} w+
\nabla^2w)
\end{equation}

And
\begin{equation}
\nabla\cdot(\bm{f}g)
=(\nabla\cdot{\bm{f}})g
+\bm{f}\cdot\nabla g
=(\nabla\cdot{\bm{f}})
(1+e^{-\lambda x}w)
+f_r  e^{-\lambda x}
(-\lambda\cos\theta w+\pd_rw)
\end{equation}

Thus Eq.\eqref{eq1} can be reformulated as
\begin{equation}
-\lambda^2 w+
\nabla^2w+(e^{\lambda r\cos\theta}+w)\pd_rf_r
+f_r
(-\lambda\cos\theta w+\pd_rw)
=0
\end{equation}
%-----------------------------


%-----------------------------
\section{Useful formulate}
\begin{equation}
\nabla f=\pd_rf\bm{\hat{e}}_r+\frac{1}{r}\pd_\theta f\bm{\hat{e}}_\theta
\end{equation}

\begin{equation}
\begin{split}
\nabla \cdot\bm{A}&=\frac{1}{r}\pd_r (rA_r)+\frac{1}{r}\pd_\theta A_\theta
\\
&=\pd_r A_r+\frac{A_r}{r}+\frac{1}{r}\pd_\theta A_\theta
\end{split}
\end{equation}

\begin{equation}
\begin{split}
\nabla^2f&=\frac{1}{r}\pd_r (r\pd_rf)+\frac{1}{r^2}\pd_\theta^2f
\\
&=\pd_r^2 f+\frac{\pd_rf}{r}+\frac{1}{r^2}\pd_\theta ^2f
\end{split}
\end{equation}

\begin{equation}
\pd_x =\cos\theta \pd_r
-\frac{\sin\theta}{r}\pd_\theta
\end{equation}
%-----------------------------





%-----------------------------
\section{Solution of $D=0$}
In the convection limit, $D=0$, the equation is reduced to
\begin{equation}
\nabla\cdot(\bm{f}g)
+u\pd_xg=0
\end{equation}

Let the radius size is $r_0=1$, $\bm{f}=-k(r-1)\Theta (1-r)
\bm{\hat{e}}_r
$

Assume that $g(r\geq1=1)$, so we focus on the regime of $r\leq1$, where
$\bm{f}=-k(r-1)\bm{\hat{e}}_r$
and

\begin{equation}
\nabla\cdot \bm{f}
=k(\frac{1}{r}-2)
\end{equation}

so
\begin{equation}
\nabla\cdot(\bm{f}g)
=k(\frac{1}{r}-2)g
-k(r-1)\pd_rg
\end{equation}
and

\begin{equation}
u\pd_xg=u\cos\theta\pd_rg
-u\frac{\sin\theta}{r}\pd_\theta g
\end{equation}

%-----------------------------

Let $g=g(r,\theta)=\xi(r)\psi(\cos\theta)=\xi(r)\psi(w),\quad w=\cos\theta$

so
\begin{equation}
k(\frac{1}{r}-2)\xi\psi
-k(r-1)\xi'\psi+uw\xi'\psi+\frac{u}{r}\xi\psi'=0
\end{equation}


\end{document}
